Shuffle path.lean around

src/graph_theory/path.lean
@@ -12,10 +12,26 @@ namespace simple_graph
     namespace path
         variables {V : Type} {G : simple_graph V} {u x y z : V}
 
-        def mem (z : V) (p : path G x y) : Prop
-            := path.rec (eq z) (λ x' _ _ _ _ ih, z = x' ∨ ih) p
+        def from_edge (h : G.adj x y) : path G x y := step h (point y)
 
-        instance : has_mem V (path G x y) := ⟨mem⟩
+        def append (p : path G x y) (h : G.adj y z) : path G x z
+            := path.rec (λ _, from_edge) (λ _ _ _ h' _ ih, step h' ∘ ih) p h
+
+        def concat (p : path G x y) (p' : path G y z) : path G x z
+            := path.rec (λ _, id) (λ _ _ _ h' _ ih, step h' ∘ ih) p p'
+
+        def mem (z : V) (p : path G x y) : Prop           := path.rec (eq z)      (λ u _ _ _ _ h, z = u ∨ h)          p
+        def size        (p : path G x y) : nat            := path.rec (λ _, 0)    (λ _ _ _ _ _ h, h + 1)              p
+        def rev         (p : path G x y) : path G y x     := path.rec (point)     (λ _ _ _ e _ h, append h (G.sym e)) p
+        def all_edges   (p : path G x y) : list (edges G) := path.rec (λ _, [])   (λ _ _ _ e _ h, ⟨e⟩ :: h)           p
+        def nodup       (p : path G x y) : Prop           := path.rec (λ _, true) (λ u _ _ _ p h, ¬ mem u p ∧ h)      p
+        def to_list     (p : path G x y) : list V         := path.rec (λ u, [u])  (λ u _ _ _ _ h, u :: h)             p
+
+        def init (p : path G x y) : list V := p.to_list.init
+        def tail (p : path G x y) : list V := p.to_list.tail
+
+        instance : has_mem    V (path G x y) := ⟨mem⟩
+        instance : has_sizeof   (path G x y) := ⟨size⟩
 
         @[simp] lemma mem_point : z ∈ (point x : path G x x) <-> z = x
             := iff.rfl
@@ -29,22 +45,11 @@ namespace simple_graph
         lemma mem_tail {p : path G x y} : y ∈ p
             := by { induction p, exact rfl, simp, right, assumption }
 
-        def size (p : path G x y) : nat
-            := path.rec (λ _, 0) (λ _ _ _ _ _, nat.succ) p
-
-        instance : has_sizeof (path G x y) := ⟨size⟩
-
         @[simp] lemma size_point : size (point x : path G x x) = 0
             := rfl
 
         @[simp] lemma size_step (p : path G x y) {h : G.adj z x} : size (step h p) = size p + 1
             := rfl
-
-        def from_edge (h : G.adj x y) : path G x y
-            := step h (point y)
-
-        def append (p : path G x y) (h : G.adj y z) : path G x z
-            := path.rec (λ _, from_edge) (λ _ _ _ h' _ ih, step h' ∘ ih) p h
 
         @[simp] lemma append_point {h : G.adj x y} : append (point x : path G x x) h = step h (point y : path G y y)
             := rfl
@@ -58,9 +63,6 @@ namespace simple_graph
         @[simp] lemma size_append {p : path G x y} {h : G.adj y z} : size (append p h) = size p + 1
             := by { induction p, refl, simp [*] }
 
-        def rev (p : path G x y) : path G y x
-            := path.rec (point) (λ _ _ _ h _ ih, append ih (G.sym h)) p
-
         @[simp] lemma rev_step {h : G.adj x y} {p : path G y z} : rev (step h p) = append (rev p) (G.sym h)
             := rfl
 
@@ -69,9 +71,6 @@ namespace simple_graph
 
         @[simp] lemma mem_rev {p : path G x y} : z ∈ rev p <-> z ∈ p
             := by { induction p, exact iff.rfl, simp [*], exact or.comm }
-
-        def concat (p : path G x y) (p' : path G y z) : path G x z
-            := path.rec (λ _, id) (λ _ _ _ h' _ ih, step h' ∘ ih) p p'
 
         @[simp] lemma concat_point {p : path G x y} : concat (path.point x) p = p
             := rfl
@@ -82,9 +81,6 @@ namespace simple_graph
         @[simp] lemma size_concat {p : path G x y} {p' : path G y z} : (concat p p').size = p.size + p'.size
             := by { induction p; simp [*], linarith }
 
-        def all_edges (p : path G x y) : list (edges G)
-            := path.rec (λ _, []) (λ _ _ _ h _, list.cons ⟨h⟩) p
-
         @[simp] lemma all_edges_point : all_edges (point x : path G x x) = []
             := rfl
 
@@ -93,13 +89,6 @@ namespace simple_graph
 
         lemma mem_edges {p : path G x y} {e : edges G} : e ∈ p.all_edges -> e.x ∈ p ∧ e.y ∈ p
             := by { induction p, simp, intro hh, simp at hh, cases hh; simp [*], right, apply mem_head }
-
-        -- lemma edges_simple {l} (h : llist.is_path G.adj l) (hs : llist.nodup l) : list.pairwise (edges.nsame) (edges_aux G l h)
-        --     := by { induction l with v v l hr, { exact list.pairwise.nil },
-        --         { apply list.pairwise.cons,
-        --         { intros e he, rw [edges.nsame, edges.same], push_neg, have h5 := mem_edges_aux he,
-        --             split; intro h6; subst h6, exact hs.1 h5.1, exact hs.1 h5.2 },
-        --         { exact hr h.2 hs.2 } } }
 
         lemma to_path (h : linked G x y) : nonempty (path G x y)
             := by { induction h with x' y' h1 h2 ih,
@@ -115,9 +104,6 @@ namespace simple_graph
         lemma iff_path : linked G x y <-> nonempty (path G x y)
             := ⟨to_path, from_path⟩
 
-        def nodup (p : path G x y) : Prop
-            := path.rec (λ _, true) (λ x _ _ _ p ih, x ∉ p ∧ ih) p
-
         @[simp] lemma nodup_point : nodup (point x : path G x x) := trivial
 
         @[simp] lemma nodup_step {h : G.adj x y} {p : path G y z} : nodup (step h p) <-> x ∉ p ∧ nodup p
@@ -129,43 +115,13 @@ namespace simple_graph
         lemma nodup_rev {p : path G x y} : nodup p -> nodup p.rev
             := by { induction p, obviously }
 
-        def to_list (p : path G x y) : list V
-            := path.rec (λ x', [x']) (λ x' _ _ _ _ ih, x' :: ih) p
-
         @[simp] def to_list_step {h : G.adj x y} {p : path G y z} : to_list (step h p) = x :: to_list p := rfl
 
-        def init (p : path G x y) : list V
-            := path.rec (λ _, []) (λ x' _ _ _ _ ih, x' :: ih) p
-
-        @[simp] lemma init_step {h : G.adj x y} {p : path G y z} : init (step h p) = x :: init p := rfl
-
-        def init' (p : path G x y) : list V := p.to_list.init
-
-        @[simp] lemma init'_step {h : G.adj x y} {p : path G y z} : init' (step h p) = x :: init' p
+        @[simp] lemma init_step {h : G.adj x y} {p : path G y z} : init (step h p) = x :: init p
             := by { cases p; refl }
-
-        example  {p : path G x y} : init p = init' p
-            := by { induction p, refl, simpa }
-
-        def tail (p : path G x y) : list V
-            := path.rec (λ _, []) (λ x' y' z' h' p' ih, to_list p') p
 
         @[simp] lemma tail_step {h : G.adj x y} {p : path G y z} : tail (step h p) = y :: tail p
-            := by { induction p with x' x' y' z' h' p' ih, refl, unfold tail, unfold to_list }
-
-        def tail' (p : path G x y) : list V
-            := path.rec (λ _, []) (λ _ y' _ _ _ ih, y' :: ih) p
-
-        @[simp] lemma tail'_step {h : G.adj x y} {p : path G y z} : tail' (step h p) = y :: tail' p := rfl
-
-        example {p : path G x y} : tail p = tail' p := by { induction p, refl, simpa }
-
-        def tail'' (p : path G x y) : list V := p.to_list.tail
-
-        @[simp] lemma tail''_step {h : G.adj x y} {p : path G y z} : tail'' (step h p) = y :: tail'' p
             := by { cases p; refl }
-
-        example {p : path G x y} : tail p = tail'' p := by { cases p; refl }
     end path
 
     @[ext] structure spath {V : Type} (G : simple_graph V) (x y : V)
@@ -183,8 +139,5 @@ namespace simple_graph
 
         def rev (p : spath G x y) : spath G y x
             := ⟨p.p.rev, path.nodup_rev p.simple⟩
-
-        -- lemma edges_simple {p : spath G x y} : list.pairwise (edges.nsame) p.to_path.all_edges
-        --     := path.edges_simple G _ p.simple
     end spath
 end simple_graph
